refocusing_lang_facts.v
@@ -4,13 +4,13 @@ Require Import Eqdep.
 
 Module RED_LANG_Facts (R : RED_LANG).
 
-    Import R.
-
-    Lemma ccons_inj : 
-        forall ec {k1 k2} (c : context k1 k2) ec' {k2'} (c' : context k1 k2'), 
-            k2 +> ec = k2' +> ec' -> ec=:c ~= ec'=:c' ->
-            ec = ec' /\ k2 = k2' /\ c ~= c'.
-    Proof.
+  Import R.
+  
+  Lemma ccons_inj : 
+      forall ec {k1 k2} (c : context k1 k2) ec' {k2'} (c' : context k1 k2'), 
+          k2 +> ec = k2' +> ec' -> ec=:c ~= ec'=:c' ->
+          ec = ec' /\ k2 = k2' /\ c ~= c'.
+  Proof.
     intros.
     assert (H1 := JMeq_eq_depT _ _ _ _ _ _ H H0).
     assert (H2 := eq_dep_eq_sigT _ _ _ _ _ _ H1). 
@@ -18,25 +18,28 @@ Module RED_LANG_Facts (R : RED_LANG).
     assert (H7' := inj_pair2 _ _ _ _ _ H7); subst; clear H7.
     assert (H7'' := inj_pair2 _ _ _ _ _ H7'); subst; clear H7'.
     auto.
-    Qed.
+  Qed.
 
-    Lemma context_tail_liveness : 
-        forall k ec, ~ dead_ckind (k+>ec) -> ~ dead_ckind k.
-    Proof.
+
+  Lemma context_tail_liveness : 
+      forall k ec, ~ dead_ckind (k+>ec) -> ~ dead_ckind k.
+  Proof.
     intuition.
     apply H.
     apply ckind_death_propagation.
     assumption.
-    Qed.
+  Qed.
 
-    Lemma proper_death2 : forall k1 k2, context k1 k2 -> redex k2 -> ~ dead_ckind k1.
-    Proof.
+
+  Lemma proper_death2 : forall k1 k2, context k1 k2 -> redex k2 -> ~ dead_ckind k1.
+  Proof.
     intuition.
     eapply proper_death;
     eauto.
-    Qed.
+  Qed.
 
-    Ltac inversion_ccons H :=
+
+  Ltac inversion_ccons H :=
 
       match type of H with ?ec1 =: ?c1  ~=  ?ec2 =: ?c2 => 
 
@@ -55,43 +58,49 @@ Module RED_LANG_Facts (R : RED_LANG).
 
       end.
 
-  Lemma plug_empty    : forall t k, plug t (@empty k) = t.
+
+  Lemma plug_empty : forall t k, plug t (@empty k) = t.
   Proof.
-  intuition.
+    intuition.
   Qed.
+
 
   Lemma compose_empty : forall {k1 k2} (c : context k1 k2), c = c ~+ [_].
   Proof.
-  induction c.
-  - trivial.
-  - simpl; rewrite <- IHc; trivial.
+    induction c.
+    - trivial.
+    - simpl; rewrite <- IHc; trivial.
   Qed.
+
 
   Lemma plug_compose  : 
       forall {k1 k2 k3} (c0 : context k1 k2) (c1 : context k3 k1) t, 
-           plug t (c0 ~+ c1) = plug (plug t c0) c1.
+          plug t (c0 ~+ c1) = plug (plug t c0) c1.
   Proof.
-  induction c0; intros.
-  - trivial.
-  - simpl; rewrite IHc0; trivial.
+    induction c0; intros.
+    - trivial.
+    - simpl; rewrite IHc0; trivial.
   Qed.
+
 
   Lemma context_snoc : forall ec0 {k1 k2} (c0 : context k1 k2),
                            exists ec1 c1, (ec0=:c0) = (c1~+ec1=:[_]).
   Proof.
-  intros; revert ec0.
-  induction c0; intros.
-  - exists ec0; eexists [_]; trivial.
-  - destruct IHc0 with ec as (ec1, (c1, IH)).
-    exists ec1; eexists (ec0=:c1); rewrite IH; trivial.
+    intros; revert ec0.
+    induction c0; intros.
+    - exists ec0; eexists [_]; trivial.
+    - destruct IHc0 with ec as (ec1, (c1, IH)).
+      exists ec1; eexists (ec0=:c1); rewrite IH; trivial.
   Qed.
 
-  Lemma dead_contex_dead : forall {k1 k2}, context k1 k2 -> dead_ckind k1 -> dead_ckind k2.
+
+  Lemma dead_contex_dead : 
+      forall {k1 k2}, context k1 k2 -> dead_ckind k1 -> dead_ckind k2.
   Proof with auto.
-  intros ? ? c H; revert c.
-  induction 1.
-  - trivial.
-  - apply ckind_death_propagation...
+    intros ? ? c H; revert c.
+    induction 1.
+    - trivial.
+    - apply ckind_death_propagation...
   Qed.
 
 End RED_LANG_Facts.
